sketch how a program logic proof could abstract over the ext_spec for IO, and instantiate squarer_correct for MMIO and syscalls

bedrock2/src/Examples/Trace.v
@@ -1,49 +1,74 @@
 Require Import Coq.ZArith.ZArith. Open Scope Z_scope.
+Require Import bbv.HexNotationZ.
+Require Import Coq.Strings.String.
 Require Import Coq.Lists.List. Import ListNotations.
 Require Import coqutil.Word.Interface.
 Require Import coqutil.Map.Interface.
+Require Import coqutil.Tactics.Tactics.
 Require Import bedrock2.ListPred. Import ListPredNotations.
 Require Import bedrock2.Semantics.
-
-(*Require Import bedrock2.BasicC64Syntax.*)
 Require Import bedrock2.Syntax.
-(*Local Existing Instance bedrock2.BasicC64Syntax.StringNames_params.*)
-
+Require Import bedrock2.NotationsInConstr.
 
 (* TODO distribute contents of this file into the right places *)
 
-Section Squarer.
+Module Squarer.
 
-  Context {p: Semantics.parameters}.
+  Class parameters := {
+    semantics_params :> Semantics.parameters;
 
-  Definition Event: Type := (mem * actname * list word) * (mem * list word).
+    (* macros to be inlined to read or write a word
+       TODO it's not so nice that we need to foresee the number of temp vars
+       each implementation might need *)
+    read_word_code(x tmp: varname): cmd;
+    write_word_code(x tmp: varname): cmd;
 
-  Context (read_word: word -> list Event -> Prop).
-  Context (write_word: word -> list Event -> Prop).
+    (* means "this trace does nothing else than reading the given word", could require
+       several events if we're polling until a word is available *)
+    read_word_trace: word -> trace -> Prop;
+    (* means "this trace does nothing else than outputting the given word", could require
+       several events if we have to poll a "ready to accept next word" flag before writing *)
+    write_word_trace: word -> trace -> Prop;
 
-  Definition squarer_trace: list Event -> Prop :=
-    (existsl (fun inp => read_word inp +++ write_word (word.mul inp inp))) ^*.
+    read_word_correct: forall t m l x tmp,
+        exec map.empty (read_word_code x tmp) t m l (fun t' m' l' =>
+          m = m' /\ exists t'' v, t' = t ++ t'' /\ read_word_trace v t'' /\ l' = map.put l x v);
 
-  Definition squarer: Syntax.cmd. Admitted.
+    write_word_correct: forall t m l x tmp v,
+        map.get l x = Some v ->
+        exec map.empty (write_word_code x tmp) t m l (fun t' m' l' =>
+          m = m' /\ exists t'', t' = t ++ t'' /\ write_word_trace v t'' /\ l' = l);
+  }.
+
+End Squarer.
+
+Section Squarer1.
+
+  Context {p: Squarer.parameters}.
+
+  Definition squarer_trace: trace -> Prop :=
+    kleene (existsl (fun inp => Squarer.read_word_trace inp +++
+                                Squarer.write_word_trace (word.mul inp inp))).
+
+  Definition squarer: cmd. Admitted.
 
   Lemma squarer_correct: forall (m: mem) (l: locals),
       exec map.empty squarer nil m l (fun t' m' l' => squarer_trace t').
   Admitted.
 
-End Squarer.
+End Squarer1.
 
 
 (* TODO: on which side of the list do we add new events? *)
 
 Module SpiEth.
 
-  Inductive actname := MMInput | MMOutput.
+  Inductive MMIOAction := MMInput | MMOutput.
 
   Section WithMem.
     Context {byte: word.word 8} {word: word.word 32} {mem: map.map word byte}.
-    (* Context {mem: Type}. *)
 
-    Definition Event: Type := (mem * actname * list word) * (mem * list word).
+    Definition Event: Type := (mem * MMIOAction * list word) * (mem * list word).
 
     Definition msb_set(x: word): Prop :=
       word.and x (word.slu (word.of_Z 1) (word.of_Z 31)) <> word.of_Z 0.
@@ -51,9 +76,19 @@ Module SpiEth.
     Definition lo_byte(x: word): word :=
       word.and x (word.of_Z 255).
 
-    (* TODO hex notation *)
-    Definition spi_rx     : word := word.of_Z 268582988. (* 0x1002404c *)
-    Definition spi_tx_fifo: word := word.of_Z 268582984. (* 0x10024048 *)
+    Definition spi_rx     : Z := Ox"1002404c".
+    Definition spi_tx_fifo: Z := Ox"10024048".
+    Definition spi_pinmux : Z := Ox"10012038".
+    Definition spi_sckdiv : Z := Ox"10024000".
+    Definition spi_csmode : Z := Ox"10024018".
+
+    (* TODO should this be so specific or should it be the whole range? *)
+    Definition isMMIOAddr(a: word): Prop :=
+      a = word.of_Z spi_rx      \/
+      a = word.of_Z spi_tx_fifo \/
+      a = word.of_Z spi_pinmux  \/
+      a = word.of_Z spi_sckdiv  \/
+      a = word.of_Z spi_csmode  .
 
     (*  // Reads one byte over SPI and returns
         static inline w spi_read() {
@@ -65,11 +100,11 @@ Module SpiEth.
     Inductive read_byte: word -> list Event -> Prop :=
     | read_byte_go: forall x m,
         ~ msb_set x ->
-        read_byte (lo_byte x) [((m, MMInput, [spi_rx]), (m, [x]))]
+        read_byte (lo_byte x) [((m, MMInput, [word.of_Z spi_rx]), (m, [x]))]
     | read_byte_wait: forall x y m rest,
         msb_set x ->
         read_byte y rest ->
-        read_byte y (((m, MMInput, [spi_rx]), (m, [x])) :: rest).
+        read_byte y (((m, MMInput, [word.of_Z spi_rx]), (m, [x])) :: rest).
 
     (*  // Requires b < 256
         static inline void spi_write(w b) {
@@ -81,12 +116,99 @@ Module SpiEth.
     | write_byte_go: forall x b m,
         ~ msb_set x ->
         0 <= b < 256 ->
-        write_byte (word.of_Z b) [((m, MMInput, [spi_tx_fifo]), (m, [x]));
-                                  ((m, MMOutput, [spi_tx_fifo; word.of_Z b]), (m, []))]
+        write_byte (word.of_Z b) [((m, MMInput, [word.of_Z spi_tx_fifo]), (m, [x]));
+                                  ((m, MMOutput, [word.of_Z spi_tx_fifo; word.of_Z b]), (m, []))]
     | write_byte_wait: forall x b m rest,
         msb_set x ->
         write_byte b rest ->
-        write_byte b (((m, MMInput, [spi_tx_fifo]), (m, [x])) :: rest).
+        write_byte b (((m, MMInput, [word.of_Z spi_tx_fifo]), (m, [x])) :: rest).
+
+
+    Instance squarer_syntax_params: Syntax.parameters := {|
+      Syntax.varname := string;
+      Syntax.funname := Empty_set;
+      Syntax.actname := MMIOAction;
+    |}.
+    Local Set Refine Instance Mode.
+
+    Context {locals: map.map varname word}.
+    Context {env: map.map funname (list varname * list varname * cmd)}.
+
+    Instance squarer_semantics_params: Semantics.parameters := {|
+      Semantics.syntax := squarer_syntax_params;
+      Semantics.width := 32;
+      Semantics.word := word;
+      Semantics.byte := byte;
+      Semantics.mem := mem;
+      Semantics.funname_eqb f1 f2 := Empty_set_rect (fun _ : Empty_set => bool) f1;
+      Semantics.ext_spec t m action (argvals: list word) (post: (mem -> list word -> Prop)) :=
+        match argvals with
+        | addr :: _ =>
+          isMMIOAddr addr /\
+          Memory.load access_size.four m addr = None /\
+          match action with
+          | MMInput => argvals = [addr] /\ forall val, post m [val]
+          | MMOutput => exists val, argvals = [addr; val] /\ post m nil
+          end
+        | nil => False
+        end;
+    |}.
+
+    Local Set Refine Instance Mode.
+    Local Coercion literal(z : Z) : Syntax.expr := Syntax.expr.literal z.
+(*  Local Coercion var(x: varname): Syntax.expr := Syntax.expr.var x.*)
+    Local Coercion var(x : @varname (@syntax squarer_semantics_params)):
+      @expr.expr (@syntax squarer_semantics_params) := Syntax.expr.var x.
+    (* TODO make coercions work *)
+    (* Set Printing Implicit. Unset Printing Notations. *)
+
+    Definition TODO{T: Type}: T. Admitted.
+
+    Instance squarer_params: Squarer.parameters := {|
+      Squarer.semantics_params := squarer_semantics_params;
+
+      (* TODO these only read a byte rather than a word *)
+      Squarer.read_word_code(x _: varname) := bedrock_func_body:(
+        x = -1 ;;
+        while (var x .& (1 << 31)) {{ cmd.interact [x] MMInput [literal spi_rx] }}
+      );
+      Squarer.write_word_code(x tmp: varname) := bedrock_func_body:(
+        cmd.interact [tmp] MMInput [literal spi_tx_fifo] ;;
+        while (var tmp .& (1 << 31)) {{ (* high order bit set means fifo is full *)
+          cmd.interact [tmp] MMInput [literal spi_tx_fifo]
+        }};;
+        cmd.interact [] MMOutput [literal spi_tx_fifo; var x]
+      );
+
+      Squarer.read_word_trace := read_byte;
+      Squarer.write_word_trace := write_byte;
+
+    |}.
+    - (* read_word_correct: *)
+      intros.
+      eapply exec.seq with
+          (mid := fun t' m' l' => t' = t /\ m' = m /\ l' = map.put l x (word.of_Z (-1))).
+      { eapply exec.set; [reflexivity|auto]. }
+      { intros. apply TODO. (* will require a loop invariant *) }
+    - (* write_word_correct: *)
+      intros.
+      (* need to show that this imperative code corresponds to the Inductive write_byte *)
+      eapply exec.seq.
+      { eapply exec.interact. (* proving that MMIO ext_spec is satisfied *)
+        - simpl. reflexivity.
+        - simpl. repeat split.
+          + unfold isMMIOAddr. auto.
+          + (* TODO interesting: How to know that memory is undefined at spi_tx_fifo? *)
+            apply TODO.
+          + apply TODO.
+        - apply TODO.
+      }
+      apply TODO.
+      Grab Existential Variables. all: intros; apply True.
+    Defined.
+
+    Definition squarer_correct := @Top.squarer_correct squarer_params.
+    Check squarer_correct.
 
   End WithMem.
 End SpiEth.
@@ -94,7 +216,7 @@ End SpiEth.
 
 Module Syscalls.
 
-  Inductive actname := Syscall.
+  Inductive SyscallAction := Syscall.
 
   (* Go models syscalls as
      func Syscall(trap, a1, a2, a3 uintptr) (r1, r2 uintptr, err Errno)
@@ -102,23 +224,97 @@ Module Syscalls.
 
   Section WithMem.
     Context {byte: word.word 8} {word: word.word 32} {mem: map.map word byte}.
-    (* Context {mem: Type}. *)
 
-    Definition Event: Type := (mem * actname * list word) * (mem * list word).
+    Definition Event: Type := (mem * SyscallAction * list word) * (mem * list word).
 
-    Definition magicValue: word. Admitted.
+    Definition magicValue: Z. Admitted.
 
     (* TODO what about failures? *)
     (* TODO what if the syscall changes the memory? Do we see the whole memory? *)
     Inductive read_word: word -> list Event -> Prop :=
     | read_word_go: forall m x ret2 err,
-        read_word x [((m, Syscall, [magicValue; magicValue; magicValue; magicValue]),
+        read_word x [((m, Syscall, [word.of_Z magicValue; word.of_Z magicValue;
+                                      word.of_Z magicValue; word.of_Z magicValue]),
                       (m, [x; ret2; err]))].
 
     Inductive write_word: word -> list Event -> Prop :=
     | write_word_go: forall m x ret1 ret2 err,
-        write_word x [((m, Syscall, [x; magicValue; magicValue; magicValue]),
+        write_word x [((m, Syscall, [x; word.of_Z magicValue;
+                                       word.of_Z magicValue; word.of_Z magicValue]),
                        (m, [ret1; ret2; err]))].
+
+
+    Instance squarer_syntax_params: Syntax.parameters := {|
+      Syntax.varname := string;
+      Syntax.funname := Empty_set;
+      Syntax.actname := SyscallAction;
+    |}.
+    Local Set Refine Instance Mode.
+
+    Context {locals: map.map varname word}.
+    Context {env: map.map funname (list varname * list varname * cmd)}.
+
+    Instance squarer_semantics_params: Semantics.parameters := {|
+      Semantics.syntax := squarer_syntax_params;
+      Semantics.width := 32;
+      Semantics.word := word;
+      Semantics.byte := byte;
+      Semantics.mem := mem;
+      Semantics.funname_eqb f1 f2 := Empty_set_rect (fun _ : Empty_set => bool) f1;
+      Semantics.ext_spec t m action (argvals: list word) (post: (mem -> list word -> Prop)) :=
+        (* TODO needs to be more precise *)
+        match argvals with
+        | [trap; a1; a2; a3] => forall r1 r2 err, post m [r1; r2; err]
+        | _ => False
+        end;
+    |}.
+
+    Local Set Refine Instance Mode.
+    Local Coercion literal(z : Z) : Syntax.expr := Syntax.expr.literal z.
+(*  Local Coercion var(x: varname): Syntax.expr := Syntax.expr.var x.*)
+    Local Coercion var(x : @varname (@syntax squarer_semantics_params)):
+      @expr.expr (@syntax squarer_semantics_params) := Syntax.expr.var x.
+    (* TODO make coercions work *)
+    (* Set Printing Implicit. Unset Printing Notations. *)
+
+    Definition TODO{T: Type}: T. Admitted.
+
+    Instance squarer_params: Squarer.parameters := {|
+      Squarer.semantics_params := squarer_semantics_params;
+
+      Squarer.read_word_code(x tmp: varname) :=
+        cmd.interact [x; tmp; tmp] Syscall [literal magicValue; literal magicValue;
+                                              literal magicValue; literal magicValue];
+
+      Squarer.write_word_code(x tmp: varname) :=
+        cmd.interact [tmp; tmp; tmp] Syscall [var x; literal magicValue;
+                                                literal magicValue; literal magicValue];
+
+      Squarer.read_word_trace := read_word;
+      Squarer.write_word_trace := write_word;
+
+    |}.
+    - (* read_word_correct: *)
+      intros.
+      eapply exec.interact with (mid := fun newM resvals =>
+         newM = m /\ exists v ignored1 ignored2, resvals = [v; ignored1; ignored2]).
+      + simpl. reflexivity.
+      + simpl. eauto.
+      + intros.
+        destruct_products.
+        subst.
+        eexists. repeat split.
+        do 2 eexists. repeat split.
+        * (* TODO direction doesn't match *)
+          apply TODO.
+        * (* TODO need to specify that some ignored1, ignored2 are updated too *)
+          apply TODO.
+    - apply TODO.
+      Grab Existential Variables. all: apply (word.of_Z 42) || apply map.empty.
+    Defined.
+
+    Definition squarer_correct := @Top.squarer_correct squarer_params.
+    Check squarer_correct.
 
   End WithMem.
 End Syscalls.
